Phi_System/IDE_CP_Reasoning1.thy
@@ -1075,7 +1075,7 @@ lemma [\<phi>reason 1200 for \<open>?S \<heavy_comma> ?x \<Ztypecolon> \<v>\<a>\
 lemma [\<phi>reason 1100 for \<open>?S\<heavy_comma> ?X \<t>\<r>\<a>\<n>\<s>\<f>\<o>\<r>\<m>\<s> ?S' \<w>\<i>\<t>\<h> ?V @action collect_clean_value ?CLEAN\<close>]:
   \<open> S \<t>\<r>\<a>\<n>\<s>\<f>\<o>\<r>\<m>\<s> S' \<w>\<i>\<t>\<h> V @action collect_clean_value CLEAN
 \<Longrightarrow> S\<heavy_comma> X \<t>\<r>\<a>\<n>\<s>\<f>\<o>\<r>\<m>\<s> S'\<heavy_comma> X \<w>\<i>\<t>\<h> V @action collect_clean_value CLEAN\<close>
-  unfolding Action_Tag_def using implies_right_frame .
+  unfolding Action_Tag_def using transformation_right_frame .
 
 lemma [\<phi>reason 1050 for \<open>?x \<Ztypecolon> \<v>\<a>\<l>[?v] ?T \<t>\<r>\<a>\<n>\<s>\<f>\<o>\<r>\<m>\<s> ?S' \<w>\<i>\<t>\<h> ?V @action collect_clean_value True\<close>]:
   \<open> x \<Ztypecolon> \<v>\<a>\<l>[v] T \<t>\<r>\<a>\<n>\<s>\<f>\<o>\<r>\<m>\<s> Void \<w>\<i>\<t>\<h> \<phi>arg.dest v \<in> (x \<Ztypecolon> T) \<and> True
